i2c/i2cScript.sml
@@ -3,59 +3,21 @@
 open HolKernel Parse boolLib bossLib;
 open byteTheory;
 open ffiTheory;
-open i2cMappingsTheory;
+open i2cMappingsTheory cheshireOracleTheory;
 
 val _ = new_theory("i2c");
 
-Definition region_start_def:
-  region_start = 0x03003000 : num
+Definition i2c_oracle_read_def:
+  i2c_oracle_read = cheshire_oracle_read i2c_eat_fnum i2c_tick i2c_read
 End
 
-Definition region_end_def:
-  region_end = 0x03004000 : num
+Definition i2c_oracle_write_def:
+  i2c_oracle_write = cheshire_oracle_write i2c_eat_fnum i2c_tick i2c_write
 End
 
 Definition i2c_oracle_def:
   (* 'a is the word size of the processor. *)
-  i2c_oracle (:'a) (s: ffiname) (st: i2c_state) [(nb: word8)] (bytes: word8 list) =
-    let
-      (* nb = 0 represents the word size of the processor. *)
-      nb' = if nb = 0w then w2n (bytes_in_word : 'a word) else w2n nb;
-      addr_offset = case s of
-        SharedMem MappedRead => 0
-      | SharedMem MappedWrite => nb'
-      | _ => 0; (* We'll return an error later on. *)
-      (* The F means little-endian; nothing else in CakeML bothers handling big-endian
-       * systems, so I won't here either. *)
-      addr_word = word_of_bytes F 0w (DROP addr_offset bytes) : 'a word;
-      addr = w2n addr_word;
-      st' = apply_fbits st;
-    in
-      (* TODO: I'm pretty sure 64-bit reads get split up into two 32-bit reads, but no
-       * sane driver should be using 64-bit accesses on 32-bit registers anyway.
-       *
-       * If we do implement it, we should use `fnums` to reorder the reads
-       * non-deterministically (use each number as an index into the list of remaining
-       * options?), and use `apply_fbits` to simulate an arbitrary delay between
-       * reads. *)
-      if addr < region_start \/ addr >= region_end \/ nb' > 4 then
-        Oracle_final FFI_failed
-      else
-        case s of
-          SharedMem MappedRead =>
-            (case i2c_read st' nb' (addr - region_start) of
-              INL outcome => Oracle_final outcome
-            | INR (notif, value) => Oracle_return (i2c_tick notif st') (TAKE nb' (word_to_bytes value F)))
-        | SharedMem MappedWrite =>
-            let
-              value = word_of_bytes F 0w (TAKE addr_offset bytes)
-            in
-              (case i2c_write st' nb' (addr - region_start) value of
-                INL outcome => Oracle_final outcome
-                (* Register writes from software take priority over ones from software, so
-                 * applying `st_upd` after `i2c_tick` is correct. *)
-              | INR (st_upd, notif) => Oracle_return (st_upd (i2c_tick notif st')) [])
-        | _ => Oracle_final FFI_failed
+  i2c_oracle (:'a) = cheshire_oracle (:'a) i2c_eat_fnum i2c_tick i2c_read i2c_write
 End
 
 val _ = export_theory();
