common/byteExtraScript.sml
@@ -1,0 +1,368 @@
+open HolKernel Parse boolLib bossLib;
+open wordsLib;
+open arithmeticTheory byteTheory dividesTheory fcpTheory listTheory wordsTheory;
+
+val _ = new_theory "byteExtra";
+
+Theorem word_to_bytes_aux_length:
+  LENGTH (word_to_bytes_aux n _ _) = n
+Proof
+  Induct_on ‘n’
+  >> simp [word_to_bytes_aux_def]
+QED
+
+Theorem word_to_bytes_length:
+  LENGTH (word_to_bytes (w: 'a word) be) = dimindex (:'a) DIV 8
+Proof
+  simp [word_to_bytes_def, word_to_bytes_aux_length]
+QED
+
+Theorem MIN_VAL_1[simp]:
+  a <= b ==> MIN a b = a
+Proof
+  simp [MIN_DEF]
+QED
+
+Theorem MIN_VAL_2[simp]:
+  b <= a ==> MIN a b = b
+Proof
+  simp [MIN_DEF]
+QED
+
+Theorem MAX_VAL_1[simp]:
+  a <= b ==> MAX a b = b
+Proof
+  simp [MAX_DEF]
+QED
+
+Theorem MAX_VAL_2[simp]:
+  b <= a ==> MAX a b = a
+Proof
+  simp [MAX_DEF]
+QED
+
+Theorem word_slice_alt_or[simp]:
+  word_slice_alt h l (a || b) = word_slice_alt h l a || word_slice_alt h l b
+Proof
+  (* FCP_ss is broken, so we have to manually write the theorems it contains. *)
+  simp [word_slice_alt_def, word_or_def, FCP_BETA, FCP_ETA, CART_EQ, LEFT_AND_OVER_OR]
+QED
+
+Theorem word_slice_alt_lsl:
+  word_slice_alt h l (w << n) = word_slice_alt (h - n) (l - n) w << n
+Proof
+  simp [word_slice_alt_def, word_lsl_def, FCP_BETA, FCP_ETA, CART_EQ]
+  >> strip_tac
+  >> Cases_on ‘i < n’
+  >- simp []
+  >- (Cases_on ‘0 < h - n’
+      >> simp [])
+QED
+
+Theorem word_slice_alt_w2w_1:
+  l >= dimindex (:'a)
+  ==> word_slice_alt h l (w2w (w: 'a word)) = 0w
+Proof
+  simp [word_slice_alt_def, w2w, FCP_BETA, FCP_ETA, CART_EQ, word_0, Cong OR_CONG]
+QED
+
+Theorem word_slice_alt_w2w_2:
+  h >= dimindex (:'a)
+  ==> word_slice_alt h 0 (w2w (w: 'a word)) = w2w w
+Proof
+  simp [word_slice_alt_def, w2w, FCP_BETA, FCP_ETA, CART_EQ]
+  >> simp [Cong AND_CONG]
+QED
+
+Theorem word_slice_alt_h_zero[simp]:
+  word_slice_alt 0 l w = 0w
+Proof
+  simp [word_slice_alt_def, FCP_BETA, FCP_ETA, CART_EQ, word_0]
+QED
+
+Theorem word_slice_alt_lsl_w2w_1:
+  h <= s \/ l >= s + dimindex (:'a)
+  ==> word_slice_alt h l (w2w (w: 'a word) << s) = 0w
+Proof
+  strip_tac
+  >- (‘h - s = 0’ by simp []
+      >> simp [word_slice_alt_lsl])
+  >- (‘l - s >= dimindex (:'a)’ by simp []
+      >> simp [word_slice_alt_lsl, word_slice_alt_w2w_1, SF WORD_ss])
+QED
+
+Theorem word_slice_alt_lsl_w2w_2:
+  l <= s /\ s + dimindex (:'a) <= h
+  ==> word_slice_alt h l (w2w (w: 'a word) << s) = w2w w << s
+Proof
+  strip_tac
+  >> ‘h - s >= dimindex (:'a)’ by simp []
+  >> ‘l - s = 0’ by simp []
+  >> simp [word_slice_alt_lsl, word_slice_alt_w2w_2]
+QED
+
+Theorem word_slice_alt_word_slice_alt:
+  word_slice_alt h1 l1 (word_slice_alt h2 l2 w) = word_slice_alt (MIN h1 h2) (MAX l1 l2) w
+Proof
+  simp [word_slice_alt_def, FCP_BETA, FCP_ETA, CART_EQ]
+  >> decide_tac
+QED
+
+Theorem word_slice_alt_dimindex:
+  word_slice_alt (MIN h (dimindex (:'a))) l (w: 'a word) = word_slice_alt h l w
+Proof
+  simp [word_slice_alt_def, FCP_BETA, FCP_ETA, CART_EQ]
+QED
+
+Theorem word_slice_alt_empty[simp]:
+  h <= l ==> word_slice_alt h l w = 0w
+Proof
+  simp [word_slice_alt_def, FCP_BETA, FCP_ETA, CART_EQ, word_0]
+  >> rpt strip_tac
+  >> spose_not_then assume_tac
+  >> simp []
+QED
+
+Theorem word_slice_alt_full[simp]:
+  dimindex (:'a) <= h ==> word_slice_alt h 0 (w: 'a word) = w
+Proof
+  simp [word_slice_alt_def, FCP_BETA, FCP_ETA, CART_EQ]
+QED
+
+Theorem word_slice_alt_adjacent:
+  word_slice_alt a b w || word_slice_alt b c w = word_slice_alt (MAX a b) (MIN b c) w
+Proof
+  simp [word_slice_alt_def, FCP_BETA, FCP_ETA, CART_EQ, word_or_def]
+  >> rpt strip_tac
+  >> Cases_on ‘i >= b’
+  >> simp []
+QED
+
+Theorem word_slice_alt_word_slice_2:
+  word_slice_alt (SUC h) l w = (h '' l) w
+Proof
+  simp [word_slice_alt_def, word_slice_def, FCP_BETA, FCP_ETA, CART_EQ, LT_SUC_LE]
+QED
+
+
+Theorem word_slice_alt_set_byte_1:
+  h <= byte_index a be \/ l >= byte_index a be + 8
+  ==> word_slice_alt h l (set_byte a b w be) = word_slice_alt h l w
+Proof
+  strip_tac
+  >> simp [set_byte_def]
+  >- simp [word_slice_alt_lsl_w2w_1, word_slice_alt_word_slice_alt]
+  >- simp [word_slice_alt_lsl_w2w_1, word_slice_alt_word_slice_alt, word_slice_alt_dimindex]
+QED
+
+Theorem word_slice_alt_set_byte_2:
+  l <= byte_index a be /\ byte_index a be + 8 <= h
+  ==> word_slice_alt h l (set_byte a b w be) = set_byte a b (word_slice_alt h l w) be
+Proof
+  simp [set_byte_def, word_slice_alt_lsl_w2w_2, word_slice_alt_word_slice_alt, MIN_COMM]
+QED
+
+Theorem lt_or_gt:
+  (a: num) <> b ==> a < b \/ a > b
+Proof
+  simp []
+QED
+
+Theorem byte_index_lt_or_gt:
+  w2n (n: 'a word) MOD (dimindex (:'a) DIV 8) <> w2n (m: 'a word) MOD (dimindex (:'a) DIV 8)
+  /\ dimindex (:'a) DIV 8 > 0
+  ==> byte_index m be >= byte_index n be + 8 \/ byte_index m be + 8 <= byte_index n be
+Proof
+  strip_tac
+  >> drule lt_or_gt
+  >> strip_tac
+  >> Cases_on ‘be’
+  >> simp [byte_index_def]
+  >> qabbrev_tac ‘bytes = dimindex (:'a) DIV 8’
+  >> ‘w2n m MOD bytes < bytes’ by simp []
+  >> ‘w2n n MOD bytes < bytes’ by simp []
+  >> simp []
+QED
+
+Theorem set_byte_independent:
+  w2n n MOD (dimindex (:'a) DIV 8) <> w2n m MOD (dimindex (:'a) DIV 8)
+  /\ dimindex (:'a) DIV 8 > 0
+  ==> set_byte n x (set_byte m y (w: 'a word) be) be = set_byte m y (set_byte n x w be) be
+Proof
+  strip_tac
+  >> drule_all_then (qspec_then ‘be’ assume_tac) byte_index_lt_or_gt
+  >> rw []
+  >> simp [Once set_byte_def, word_slice_alt_set_byte_1]
+  >> simp [Once set_byte_def, word_slice_alt_set_byte_1]
+  >> simp [Once set_byte_def, word_slice_alt_set_byte_1]
+  >> simp [Once set_byte_def, word_slice_alt_set_byte_1]
+  >> simp [word_slice_alt_word_slice_alt]
+  >> qspecl_then [‘1’, ‘dimindex (:'a)’, ‘8’] assume_tac X_LE_DIV
+  >> ‘8 <= dimindex (:'a)’ by simp []
+  >> simp [byte_index_offset, word_slice_alt_lsl_w2w_2, MIN_COMM]
+QED
+
+Theorem w2n_add_2:
+  w2n (a: 'a word) + w2n b < dimword (:'a) ==> w2n (a + b) = w2n a + w2n b
+Proof
+  simp [word_add_def]
+QED
+
+Theorem word_of_bytes_SNOC:
+  !n. LENGTH bs < dimindex (:'a) DIV 8 /\ w2n (n: 'a word) + LENGTH bs < dimword (:'a)
+      ==> word_of_bytes be n (SNOC b bs) = set_byte (n + n2w (LENGTH bs)) b (word_of_bytes be n bs) be
+Proof
+  Induct_on ‘bs’
+  >- simp [word_of_bytes_def]
+  >- (rpt strip_tac
+      >> last_x_assum (qspec_then ‘n + 1w’ mp_tac)
+      >> impl_tac
+      (* Seems like only fs will rewrite assumptions. *)
+      >- fs [w2n_add_2]
+      >- (fs [word_of_bytes_def, ADD1, GSYM word_add_n2w]
+          >> strip_tac
+          >> irule set_byte_independent
+          >> simp [w2n_add_2]
+          >> ‘0 < dimindex (:'a) DIV 8’ by simp []
+          >> dxrule_then (qspecl_then [‘LENGTH bs + 1’, ‘0’, ‘w2n n’] assume_tac) ADD_MOD
+          >> simp [Once EQ_SYM_EQ]
+          >> fs []))
+QED
+
+Theorem word_of_bytes_0_SNOC:
+  LENGTH bs < dimindex (:'a) DIV 8
+  ==> word_of_bytes be 0w (SNOC b bs): 'a word = set_byte (n2w (LENGTH bs)) b (word_of_bytes be 0w bs) be
+Proof
+  strip_tac
+  >> ‘dimindex (:'a) DIV 8 <= dimindex (:'a)’ by simp [DIV_LESS_EQ]
+  >> simp [dimindex_lt_dimword, LESS_LESS_EQ_TRANS, LESS_TRANS, word_of_bytes_SNOC]
+QED
+
+Theorem word_bits_dimindex:
+  (MIN h (dimindex (:'a) - 1) -- l) (w: 'a word) = (h -- l) w
+Proof
+  Cases_on ‘h > dimindex (:'a) - 1’
+  >- simp [WORD_BITS_MIN_HIGH]
+  >- simp []
+QED
+
+Theorem word_bits_lsr_2:
+  (h -- l) (w >>> n) = (h + n -- l + n) w
+Proof
+  simp [word_lsr_n2w, WORD_BITS_COMP_THM, MIN_COMM, word_bits_dimindex]
+QED
+
+Theorem word_of_bytes_word_to_bytes_aux_le:
+  n <= dimindex (:'a) DIV 8 /\ 8 <= dimindex (:'a)
+  ==> word_of_bytes F 0w (word_to_bytes_aux n (w: 'a word) F) = word_slice_alt (8 * n) 0 w
+Proof
+  Induct_on ‘n’
+  >- simp [word_to_bytes_aux_def, word_of_bytes_def]
+  >- (strip_tac
+      >> ‘dimindex (:'a) DIV 8 <= dimindex (:'a)’ by simp [DIV_LESS_EQ]
+      >> ‘n < dimword (:'a)’ by simp [dimindex_lt_dimword, LESS_TRANS, LESS_LESS_EQ_TRANS]
+      (* The n < dimword (:'a) happens to be needed for reasons other than word_of_bytes_SNOC, so there's no point in switching to word_of_bytes_0_SNOC. *)
+      >> simp [word_to_bytes_aux_def, GSYM SNOC_APPEND, word_to_bytes_aux_length, word_of_bytes_SNOC, set_byte_def, get_byte_def, word_slice_alt_word_slice_alt, byte_index_def, w2w_w2w, word_bits_lsr_2, GSYM WORD_SLICE_THM]
+      >> qspecl_then [‘SUC n’, ‘dimindex (:'a)’, ‘8’] assume_tac X_LE_DIV
+      >> rfs [GSYM word_slice_alt_word_slice, word_slice_alt_adjacent, ADD1]
+      >> simp [GSYM ADD1, MULT_CLAUSES])
+QED
+
+(* TODO: big-endian *)
+(* The fact that the divides 8 (dimindex (:'a)) is necessary is arguably a bug in word_to_bytes. *)
+Theorem word_to_bytes_word_of_bytes_le:
+  8 <= dimindex (:'a) /\ divides 8 (dimindex (:'a))
+  ==> word_of_bytes F 0w (word_to_bytes (w: 'a word) F) = w
+Proof
+  simp [word_to_bytes_def, word_of_bytes_word_to_bytes_aux_le, DIVIDES_DIV]
+QED
+
+Theorem set_byte_unchanged:
+  (byte_index a be + 7 -- byte_index a be) w = w2w b
+  ==> set_byte a b w be = w
+Proof
+  disch_then (assume_tac o GSYM)
+  >> simp [set_byte_def, GSYM WORD_SLICE_THM, GSYM word_slice_alt_word_slice_2, ADD1, word_slice_alt_adjacent]
+QED
+
+(* TODO: I think proving all these theorems about word_slice_alt was a mistake, it was only defined to make the definition of set_byte a little nicer.
+ *
+ * Sure, use it for the ones where supporting zero-length slices is actually key to the theorem being correct, but use the regular ones everywhere you can and convert between them.
+ *
+ * I think this one may be an example of where word_slice_alt makes sense: it would be weaker if described using '', since it couldn't express the case where bs is 0 elements long. *)
+Theorem word_of_bytes_msb:
+  !n bs h l.
+    l >= 8 * (w2n n + LENGTH bs)
+    ==> word_slice_alt h l (word_of_bytes F n bs: 'a word) = 0w
+Proof
+  Induct_on ‘bs’
+  >- simp [word_of_bytes_def, word_slice_alt_zero]
+  >- (rpt strip_tac
+      >> Cases_on ‘dimindex (:'a) < 8 * (w2n n + 1)’
+      >- (fs [Once (GSYM word_slice_alt_dimindex), LESS_LESS_EQ_TRANS, LESS_EQ_TRANS])
+      >- (first_x_assum (qspec_then ‘n + 1w’ assume_tac)
+          >> qspecl_then [‘8’, ‘8 * (w2n n + 1)’, ‘dimindex (:'a)’] assume_tac DIV_LE_MONOTONE
+          >> rfs [NOT_LESS, dimindex_lt_dimword, w2n_add_2, ADD1, word_of_bytes_def, byte_index_def, word_slice_alt_set_byte_1]))
+QED
+
+Theorem word_bits_word_slice_lsr:
+  (h -- l) (w: 'a word) = (h '' l) w >>> l
+Proof
+  simp [word_bits_def, word_slice_def, word_lsr_def, FCP_BETA, FCP_ETA, CART_EQ, Cong AND_CONG, SUB_LESS_OR_EQ]
+  >> decide_tac
+QED
+
+Theorem word_bits_word_slice_0:
+  (h -- l) w = 0w <=> (h '' l) w = 0w
+Proof
+  iff_tac
+  >- simp [WORD_SLICE_THM]
+  >- simp [word_bits_word_slice_lsr]
+QED
+
+(* TODO: remove this and all the other theorems that aren't needed now that we slice the value before passing it into `word_to_bytes`.
+ * I'm going to commit them first so that they're preserved in the commit history. *)
+Theorem word_of_bytes_PAD_RIGHT_zero:
+  n <= dimindex (:'a) DIV 8
+  ==> word_of_bytes F 0w (PAD_RIGHT 0w n bs): 'a word = word_of_bytes F 0w bs
+Proof
+  Induct_on ‘n’
+  >- simp [PAD_RIGHT]
+  >- (strip_tac
+      >> fs [PAD_RIGHT, SUB]
+      >> IF_CASES_TAC
+      >- simp []
+      >- (‘(byte_index (n2w n: 'a word) F + 7 -- byte_index (n2w n: 'a word) F) (word_of_bytes F 0w bs) = w2w (0w: word8): 'a word’
+            suffices_by simp [GENLIST, APPEND_SNOC, word_of_bytes_0_SNOC, set_byte_unchanged]
+          >> ‘dimindex (:'a) DIV 8 * 8 <= dimindex (:'a)’ by simp [DIV_MULT_LE]
+          >> ‘8 * n < dimindex (:'a)’ by simp []
+          >> qspec_then ‘0w’ assume_tac word_of_bytes_msb
+          >> fs [byte_index_def, dimindex_lt_dimword, word_bits_word_slice_0, GSYM word_slice_alt_word_slice_2]))
+QED
+
+Theorem set_byte_word_slice_alt_l:
+  byte_index a be <= l1 /\ l1 <= byte_index a be + 8 /\ byte_index a be <= l2 /\ l2 <= byte_index a be + 8
+  ==> set_byte a b (word_slice_alt h l1 w) be = set_byte a b (word_slice_alt h l2 w) be
+Proof
+  simp [set_byte_def, word_slice_alt_word_slice_alt]
+QED
+
+Theorem word_of_bytes_TAKE:
+  w2n m + n <= dimindex (:'a) DIV 8
+  ==> word_of_bytes F m (TAKE n bs): 'a word = word_slice_alt (8 * (w2n m + n)) (8 * w2n m) (word_of_bytes F m bs)
+Proof
+  qid_spec_tac ‘n’
+  >> qid_spec_tac ‘m’
+  >> Induct_on ‘bs’
+  >- simp [TAKE_def, word_of_bytes_def, word_slice_alt_zero]
+  >- (rpt strip_tac
+      >> simp [TAKE_def]
+      >> IF_CASES_TAC
+      >- simp [word_of_bytes_def]
+      >- (simp [word_of_bytes_def, byte_index_def, word_slice_alt_set_byte_2]
+          >> last_x_assum (qspecl_then [‘m + 1w’, ‘n - 1’] assume_tac)
+          >> ‘dimindex (:'a) DIV 8 <= dimindex (:'a)’ by simp [DIV_LESS_EQ]
+          >> gs [dimindex_lt_dimword, LESS_EQ_TRANS, LESS_EQ_LESS_TRANS, w2n_add_2, byte_index_def, set_byte_word_slice_alt_l]))
+QED
+
+val _ = export_theory ();
