common/cheshireOracleScript.sml
@@ -1,0 +1,61 @@
+open HolKernel Parse boolLib bossLib;
+open sharedMemoryOracleTheory;
+
+val _ = new_theory "cheshireOracle";
+
+(* Simulates an unknown amount of time passing, using `fnums` to determine the
+ * amount of time elapsed. *)
+Definition cheshire_wait_def:
+  cheshire_wait eat_fnum tick st =
+  let
+    (st', ticks) = eat_fnum st
+  in
+    FUNPOW (tick NONE) ticks st'
+End
+
+Definition cheshire_oracle_read_def:
+  cheshire_oracle_read
+    (eat_fnum: 'ffi -> 'ffi # num)
+    (tick: 'notif option -> 'ffi -> 'ffi)
+    (read: 'ffi -> num -> num -> ffi_outcome + 'notif option # word32)
+    (st: 'ffi) (nb: num) (addr: num) =
+  let
+    st' = cheshire_wait eat_fnum tick st;
+  in
+    if nb > 4 then
+      INL FFI_failed
+    else
+      case read st' nb addr of
+        INL outcome => INL outcome
+      | INR (notif, value) => INR (tick notif st', w2n value)
+End
+
+Definition cheshire_oracle_write_def:
+  cheshire_oracle_write
+    (eat_fnum: 'ffi -> 'ffi # num)
+    (tick: 'notif option -> 'ffi -> 'ffi)
+    (write: 'ffi -> num -> num -> word32 -> ffi_outcome + ('ffi -> 'ffi) # 'notif option)
+    (st: 'ffi) (nb: num) (addr: num) (value: num) =
+  let
+    st' = cheshire_wait eat_fnum tick st;
+  in
+    if nb > 4 then
+      INL FFI_failed
+    else
+      case write st' nb addr (n2w value) of
+        INL outcome => INL outcome
+      | INR (st_upd, notif) => INR (st_upd (tick notif st'))
+End
+
+Definition cheshire_oracle_def:
+  cheshire_oracle (:'a)
+    (eat_fnum: 'ffi -> 'ffi # num)
+    (tick: 'notif option -> 'ffi -> 'ffi)
+    (read: 'ffi -> num -> num -> ffi_outcome + 'notif option # word32)
+    (write: 'ffi -> num -> num -> word32 -> ffi_outcome + ('ffi -> 'ffi) # 'notif option) =
+  sh_mem_oracle (:'a)
+    (cheshire_oracle_read eat_fnum tick read)
+    (cheshire_oracle_write eat_fnum tick write)
+End
+
+val _ = export_theory ();
