common/sharedMemoryOracleScript.sml
@@ -1,0 +1,177 @@
+open HolKernel Parse boolLib bossLib;
+open wordsLib;
+open arithmeticTheory;
+open ffiTheory panSemTheory;
+open byteExtraTheory;
+
+val _ = new_theory "sharedMemoryOracle";
+
+Definition interp_nb_def:
+  (* nb = 0 represents the word size of the processor. *)
+  interp_nb (:'a) nb = if nb = 0 then dimindex (:'a) DIV 8 else nb
+End
+
+Definition sh_mem_oracle_def:
+  (* 'a is the word size of the processor. *)
+  sh_mem_oracle (:'a)
+    (read: 'ffi -> num -> num -> ffi_outcome + 'ffi # num)
+    (write: 'ffi -> num -> num -> num -> ffi_outcome + 'ffi)
+    (s: ffiname) (st: 'ffi) (conf: word8 list) (bytes: word8 list) =
+    let
+      nb = HD conf;
+      nb' = interp_nb (:'a) (w2n nb);
+      addr_offset = case s of
+        SharedMem MappedRead => 0
+      | SharedMem MappedWrite => nb'
+      | _ => 0; (* We'll return an error later on. *)
+      (* The F means little-endian: little-endian is used to encode shared-memory I/O regardless of the processor's endianness. *)
+      addr = word_of_bytes F 0w (DROP addr_offset bytes): 'a word;
+    in
+      case s of
+        SharedMem MappedRead =>
+          (case read st nb' (w2n addr) of
+            INL outcome => Oracle_final outcome
+          | INR (st', value) => Oracle_return st' (word_to_bytes ((8 * nb' - 1 -- 0) (n2w value: 'a word)) F))
+      | SharedMem MappedWrite =>
+          let
+            value = word_of_bytes F 0w (TAKE addr_offset bytes): 'a word;
+          in
+            (case write st nb' (w2n addr) (w2n value) of
+              INL outcome => Oracle_final outcome
+            | INR st' => Oracle_return st' (GENLIST (K 0w) (LENGTH bytes)))
+      | _ => Oracle_final FFI_failed
+End
+
+(*
+Theorem sh_mem_oracle_length:
+  sh_mem_oracle (:'a) read write s st conf bytes = Oracle_return st' bytes'
+    /\ LENGTH bytes >= interp_nb (:'a) (w2n (HD conf))
+    ==> LENGTH bytes' = LENGTH bytes
+Proof
+  simp [sh_mem_oracle_def]
+  >> rpt TOP_CASE_TAC
+  >> strip_tac
+  >> qpat_x_assum ‘_ = bytes'’ (assume_tac o GSYM)
+  >- (simp [PAD_RIGHT, LENGTH_APPEND]
+      >> ‘LENGTH (TAKE (interp_nb (:'a) (w2n (HD conf))) (word_to_bytes (n2w r: 'a word) F)) <= interp_nb (:'a) (w2n (HD conf))’ by simp [LENGTH_TAKE_EQ]
+      >> simp [])
+  >- simp []
+QED
+
+Theorem sh_mem_oracle_read_length:
+  sh_mem_oracle (:'a) read write (SharedMem MappedRead) st [nb] (word_to_bytes (addr: 'a word) F) = Oracle_return st' bytes'
+  /\ dimindex (:'a) DIV 8 >= w2n nb
+  ==> LENGTH bytes' = LENGTH (word_to_bytes (addr: 'a word) F)
+Proof
+  strip_tac
+  >> irule sh_mem_oracle_length
+  >> first_x_assum $ irule_at Any
+  >> rw [interp_nb_def, word_to_bytes_length]
+QED
+
+Theorem sh_mem_oracle_read_word_length:
+  sh_mem_oracle (:'a) read write (SharedMem MappedRead) st [0w] (word_to_bytes (addr: 'a word) F) = Oracle_return st' bytes'
+  ==> LENGTH bytes' = LENGTH (word_to_bytes (addr: 'a word) F)
+Proof
+  strip_tac
+  >> irule sh_mem_oracle_read_length
+  >> first_x_assum $ irule_at Any
+  >> simp []
+QED
+*)
+
+Theorem sh_mem_oracle_read_Oracle_return:
+  sh_mem_oracle (:'a) read write (SharedMem MappedRead) st [nb] (word_to_bytes (addr: 'a word) F) = Oracle_return st' bytes'
+  /\ 8 <= dimindex (:'a)
+  /\ divides 8 (dimindex (:'a))
+  ==> ?value. read st (interp_nb (:'a) (w2n nb)) (w2n addr) = INR (st', value)
+              /\ bytes' = word_to_bytes ((8 * interp_nb (:'a) (w2n nb) - 1 -- 0) (n2w value: 'a word)) F
+Proof
+  strip_tac
+     (* sh_mem_oracle needs to be in the goal for CASE_TAC to apply to it. *)
+  >> last_x_assum mp_tac
+  >> simp [sh_mem_oracle_def, word_to_bytes_word_of_bytes_le]
+  >> rpt CASE_TAC
+QED
+
+Theorem sh_mem_oracle_read_Oracle_final:
+  8 <= dimindex (:'a)
+  /\ divides 8 (dimindex (:'a))
+  ==> (sh_mem_oracle (:'a) read write (SharedMem MappedRead) st [nb] (word_to_bytes (addr: 'a word) F) = Oracle_final outcome
+     <=> read st (interp_nb (:'a) (w2n nb)) (w2n addr) = INL outcome)
+Proof
+  strip_tac
+  >> simp [sh_mem_oracle_def, word_to_bytes_word_of_bytes_le]
+  >> iff_tac
+  >- rpt CASE_TAC
+  >- simp []
+QED
+
+Theorem sh_mem_load_sh_mem_oracle:
+  s.ffi.oracle = sh_mem_oracle (:'a) read write
+  /\ (if nb = 0 then addr else byte_align addr) IN s.sh_memaddrs
+  /\ 32 <= dimindex (:'a)
+  /\ divides 8 (dimindex (:'a))
+  /\ nb <= 4
+  ==> sh_mem_load v (addr: 'a word) nb s =
+    let
+      nm = SharedMem MappedRead;
+      conf = [n2w nb];
+      bytes = word_to_bytes addr F;
+      nb' = interp_nb (:'a) nb;
+    in
+      case read s.ffi.ffi_state nb' (w2n addr) of
+        (* TODO: this should probably be constrained to 'a result inside CakeML, not here. *)
+        INL outcome => (SOME (FinalFFI (Final_event nm conf bytes outcome): 'a result), empty_locals s)
+      | INR (st', value) =>
+          let
+            value' = (8 * nb' - 1 -- 0) (n2w value);
+            bytes' = word_to_bytes value' F;
+          in (
+            NONE,
+            (set_var v (ValWord value') s) with ffi := s.ffi with <|
+              ffi_state := st';
+              io_events := s.ffi.io_events ++ [IO_event nm conf (ZIP (bytes, bytes'))];
+            |>
+          )
+Proof
+  simp [sh_mem_load_def, call_FFI_def]
+  >> Cases_on ‘nb = 0’
+  >> simp []
+  >> (CASE_TAC
+      >- (drule sh_mem_oracle_read_Oracle_return
+          >> rpt strip_tac
+          >> ‘32 DIV 8 <= dimindex (:'a) DIV 8’ by simp [DIV_LE_MONOTONE]
+          >> fs []
+          >> ‘1 <= interp_nb (:'a) nb’ by simp [interp_nb_def]
+          >> rfs [word_to_bytes_length, word_to_bytes_word_of_bytes_le])
+      >- (strip_tac
+          >> fs [sh_mem_oracle_read_Oracle_final]))
+QED
+
+Definition offset_oracle_read_def:
+  offset_oracle_read (base: num) read st nb addr =
+  if addr < base then
+    INL FFI_failed
+  else
+    read st nb (addr - base)
+End
+
+Definition offset_oracle_write_def:
+  offset_oracle_write (base: num) write st nb addr value =
+  if addr < base then
+    INL FFI_failed
+  else
+    write st nb (addr - base) value
+End
+
+Definition offset_oracle_def:
+  offset_oracle (:'a) base read write =
+  sh_mem_oracle (:'a) (offset_oracle_read base read) (offset_oracle_write base write)
+End
+
+Definition offset_addrs_def:
+  offset_addrs (base: 'a word) (addrs: 'a word set) = IMAGE (\addr. base + addr) addrs
+End
+
+val _ = export_theory ();
